Coq/src/drf/DRF_SC.v
@@ -28,6 +28,7 @@ Admitted.
 
 Theorem drf_sc P S X
         (nInitProg : ~ IdentMap.In tid_init P)
+        (PP : ProgLoc.prog_locs (stable_prog_to_prog P) <> [])
         (RA_RACE_FREE : sc_ra_race_free_program_G (stable_prog_to_prog P))
         (EXEC : program_execution P S X) :
   sc_consistent_ex S X.
@@ -37,7 +38,7 @@ Proof.
     apply ra_race_free_G_in_rlx_race_free_G.
     apply RA_RACE_FREE; auto.
     eby eapply drf_rc11_sc. }
-  specialize (drf_rlx nInitProg EXEC RLX_RACE_FREE) as RC11_ex.
+  specialize (drf_rlx nInitProg PP EXEC RLX_RACE_FREE) as RC11_ex.
   cdes RC11_ex.
   eexists. splits; eauto.
   eby eapply drf_rc11_sc.
